\documentclass{article}
\usepackage[utf8]{inputenc}
\usepackage{hyperref}

\title{PDE}
\author{waluigi120 }
\date{April 2018}

\begin{document}

\maketitle

\section{First-order Linear Equation}

\subsection{A simplest example}
$$\frac {\partial u} {\partial x} = 0$$
$$\Rightarrow <1,0> \cdot <u_x,u_y> = 0$$
$$\Rightarrow y = c$$

\begin{equation}\label{eq1}
u(x,y) = f(y)
\end{equation}
where f is arbitrary


\subsection{The constant coefficient equation}

Definition:
$$au_x+bu_y=0, a^2+b^2 > 0$$

Solutions:

\subsubsection{Geometric Method}

$$<a,b> \cdot <u_x,u_y> = 0$$

So $<u_x,u_y>$ is orthogonal to $<a,b>$. Since $<u_x,u_y>$ is the gradient of $u$, the function $u$ along the direction $<a,b>$ should be constant.  $bx-ay$ remains constant. It is named as characteristic line.

Similar to $(1)$, $u = f(bx-ay)$

\subsubsection{Coordinate Method}

Change variables 

\begin{equation} 
 x' = ax+by, y' = bx-ay
\end{equation}

Then by chain rule,
$$u_x = \frac{\partial u}{\partial x} = \frac{\partial u}{\partial x'} \frac{\partial x'} {\partial x} + \frac{\partial u}{\partial y'} \frac{\partial y'} {\partial x}  = a u_{x'} + b u_{y'}$$

Similiarily,
$$u_y = bu_{x'} - a u_{y'}$$

Obviously by the constant coefficient equation,
$$au_x+bu_y=(a^2+b^2)u_{x'} = 0$$

Therefore, the problem is reduced to 
$$u_{x'} = 0$$

\subsubsection{Problems}
1. Solve the PDE $4u_x - 3 u_y = 0$ with condition $u(0,y) = y^3$

Solution:

$<4,-3> \cdot <u_x.u_y> = 0 \rightarrow 3x+4y = c \rightarrow u(x,y) = f(3x+4y)$ 

$u(0,y) = y^3 \rightarrow u(0,y) = f(4y)=y^3,f(u)=(\frac{u}{4})^3$

Overall, $f(3x+4y) = \frac{(3x+4y)^3}{64}$

\subsection{The variable coefficient equation}
Definition

\begin{equation} \label{eq2}
u_x+yu_y =0
\end{equation}


It is linear (no $u^2$) and homogeneous (right hand side is zero).

One way to solve it:

Since the gradient's dot product with $<1,y>$ is zero, $<1,y>$ is tangent to the curve. 

$$\frac{dy}{dx} = y \rightarrow y = Ce^x$$

$y = Ce^x$ is called characteristic curve

Similar to the constant coefficient equation, the solution to the problem is $u(x,y) = f(C) = f(ye^{-x})$

\subsubsection{Problems}

1.Solve $u_x+2xy^2u_y=0$

Solution:

$<1,2xy^2> \cdot <u_x,u_y>=0 \rightarrow \frac{dy}{dx} = 2xy^2 \rightarrow \frac{dy}{y^2} = 2x dx \rightarrow -y^{-1} = x^2 + C \rightarrow C = -y^{-1}-x^2$

So $u(x,y) = f(y^{-1}+x^2)$

\subsection{Problems of section 1}

1. Solve $3u_y+u_{xy} = 0$

Solution:

Let $v = u_y$, 

$3v + v_x = 0 \rightarrow \frac{dv}{dx} = -3v \rightarrow v = f(y) e^{-3x}$

$u = g(y)e^{-3x} + h(x)$

2. Solve $\sqrt{1-x^2} u_x + u_y =0$, whose initial condition is $u(0,y) = y$

$\sqrt{1-x^2} u_x + u_y =0 \rightarrow <\sqrt{1-x^2},1> \cdot \nabla u = 0 \rightarrow \frac{dy}{dx} = \frac{1}{\sqrt{1-x^2}}$

$$ \int \frac{1}{\sqrt{1-x^2}} dx$$

Let $x = sin(\theta), dx = cos(\theta) d\theta, 1-x^2 = cos^2(\theta)$

$$ \int \frac{1}{cos(\theta)} cos(\theta) d\theta = \arcsin(x)$$

$\frac{dy}{dx} = \frac{1}{\sqrt{1-x^2}} \rightarrow y = \arcsin(x) + C \rightarrow u(x,y) = f(y-\arcsin(x))$

$u(0,y) = y \rightarrow u(x,y) = y-\arcsin(x)$

3.
https://math.stackexchange.com/questions/729165/finding-the-uniquely-determined-region-of-a-pde

4.Solve $au_x+bu_y +c u =0$

$au_x/u+bu_y/u +c  =0$

Let $v = \ln(u),$

$av_x+bv_y +c  =0$

Let $x' = ax+by, y' = bx-ay$

$v_x = av_{x'}+bv_{y'}, v_y = bv_{x'} -av_{y'}$

So $av_x+bv_y +c  =0 \rightarrow (a^2+b^2)v_{x'} + c =0 \rightarrow v = \frac{-cx'}{a^2+b^2} + g(bx-ay)$

$u = f(bx-ay) e^{\frac{-c(ax+by)}{a^2+b^2}}$

5. Solve $u_x+u_y+u = e^{x+2y}, u(x,0)=0$

$$\frac{dx}{1} = \frac{dy}{1} = \frac{du}{e^{x+2y}-u}$$

$\frac{dx}{1} = \frac{dy}{1} \rightarrow y=x+C$

$$\frac{du}{e^{x+2y}-u} = \frac{dx}{1}\rightarrow  \frac{du}{dx} = e^{x+2y} -u \rightarrow \frac{du}{dx} + u =  e^{x+2y} \rightarrow e^{x}\frac{du}{dx} + e^{x}u = e^{2x+2y}$$
$$\rightarrow \frac{e^{x} du}{dx} =   e^{2x+2(x+C)} \rightarrow {e^{x} u} =   \frac{1}{4}e^{2x+2y}+ C_1 = {e^{x} u} =   \frac{1}{4}e^{2x+2y}+ f(y-x) $$

$$ u = \frac{1}{4}e^{x+2y} + \frac{f(y-x)}{e^x}$$

By initial condition

$u(x,0) = \frac{1}{4}e^{x} + \frac{f(-x)}{e^x} = 0 \rightarrow f(x) = -\frac{1}{4}e^{-2x}$

$u = \frac{1}{4}e^{x+2y} - \frac{1}{4}e^{x-2y}$

6. Solve $au_x+bu_y = f(x,y)$

$$\frac{dx}{a} = \frac{dy}{b} = \frac{du}{f(x,y)}$$

$\frac{dx}{a} = \frac{dy}{b} \rightarrow bx = ay+C \rightarrow x = \frac{a}{b} y + C$

$\frac{dy}{b} = \frac{du}{f(x,y)} \rightarrow du  = \frac{f(\frac{a}{b} y + C,y)}{b} dy$

By arc length, $ds = \sqrt{1+(\frac{dx}{dy})^2} dy = \sqrt{1+(a/b)^2} dy$

So $u = \frac{1}{\sqrt{b^2+a^2}} \int f ds+C_1$

7. Solve $u_x+2u_y+(2x-y)u = 2x^2+3xy-2y^2$

Use coordinate method, (Lagrange's method is long and tedious)

$x' = x+2y,y'=2x-y,u_{x} = u_{x'}+2u_{y'},u_{y} = 2u_{x'}-u_{y'}$

$x' = <1,2>, y'=<2,-1>, 2x'-y'=<2,4>-<2,-1>=<0,5> = 5y$

$y = \frac{2}{5} x' - \frac{1}{5} y', x = x' - (\frac{4}{5} x' - \frac{2}{5} y') = \frac{1}{5} x' + \frac{2}{5} y'$

The PDE is converted to 

$u_{x'}+2u_{y'} +(2x-y)u = u_{x'}+2u_{y'}+ 2(2u_{x'}-u_{y'}) + (2(\frac{1}{5} x' + \frac{2}{5} y')-(\frac{2}{5} x' - \frac{1}{5} y'))u = 2(\frac{1}{5} x' + \frac{2}{5} y')^2+3(\frac{1}{5} x' + \frac{2}{5} y')(\frac{2}{5} x' - \frac{1}{5} y')-2(\frac{2}{5} x' - \frac{1}{5} y')^2 $

After simple algebra,

$$ (5u_{x'}+ y'u) = x'y'$$

And then it is reduced to a calculus 4 question

\section{Flows, Vibrations, and diffusions}

\subsection{Simple Transport}
Equation:

$$u_t + cu_x = 0 $$

Solution:
$$u_t + cu_x = 0 \rightarrow <1,c> \cdot \nabla = 0 \rightarrow u = f(ct-x)$$

If $x$ is fixed, as $t$ increases, $u=f(ct-x) = f(-(x-ct)) = g(x-ct)$

We can set $t=0$, and $t = 1$ to see the tendency of the graph.

When $t =0$, $u = g(x)$, consider the point $(1,g(1))$, it's right now on the position where $x=1$

When $t =1$, $u = g(x-c)$, if $u = g(1)$, then $x = c+1$, so the graph is moving toward right, by the linear transformation of the function parameters.

The velocity is defined by the displacement's difference over the time, which is $c$.

Derivation of the equation:

Assume that mass at position $[0,b]$ dissipating to $[0+ch,b+ch]$ after $\Delta t = h$
$$M = \int_0^b u(x,t) dx = \int_{ch}^{b+ch} u(x,t+h) dx $$

Differentiating with respect to $b$,

$$ u(b,t)  =  u(b+ch,t+ h) $$

Differentiating with respect to $h$,

$$ 0 = \frac{\partial u}{\partial x}\frac{\partial x}{\partial h} + \frac{\partial u}{\partial t}\frac{\partial t}{\partial h}= cu_x+u_t$$



\subsection{Vibrating String}

Preparatory:

1) Newton's second law: $F = ma$, or more precisely, $F = mu_{tt}$, u is the displacement

2) The mass of a string is the product of the density and the length.

3) The binomial expansion of square root: $(1+k)^{0.5} = 1^{0.5} \times k^0 + {0.5 \choose 1} k^1 + {0.5 \choose 2} k^2 + {0.5 \choose 3} k^3 + ...  $

As ${a \choose b} = \frac{\Gamma(a+1)}{\Gamma(b+1)\Gamma(b-a+1)}$

${0.5 \choose 1} = \frac{\Gamma(0.5+1)}{\Gamma(1+1)\Gamma(0.5-1+1)} = \frac{1}{2}$

${0.5 \choose 2} = \frac{\Gamma(0.5+1)}{\Gamma(2+1)\Gamma(0.5-2+1)} = \frac{0.5 \cdot (-0.5)}{2} = -0.125$
....

4) the portion of integration over the interval is the value of the point, as the interval goes smaller:

$$\frac{\int_a^{a+h} f dx}{a+h-a} = f(a), h \rightarrow 0$$

5)the equation for the tension along the longitudinal and traverse lines, respectively (by 1,2, and geometry):

$$\frac{T}{\sqrt{1+u_x^2}}\Big|_{x_0}^{x_1} = 0$$ 

$$\frac{Tu_x}{\sqrt{1+u_x^2}}\Big|_{x_0}^{x_1} = \int_{x_0}^{x_1} \rho u_{tt} dx$$ 

\subsubsection{Derivation of the equation, assume that the $|u_x|$ is pretty small. }

$\sqrt{1+u_x^2} = 1 + \frac{1}{2} u_x^2 - \frac{1}{8}u_x^4 + ...$

Since $|u_x|$ is pretty small, $\sqrt{1+u_x^2} \rightarrow 1$

The equations in $(5)$ becomes,

$T |_{x_0}^{x_1} = T(x_1)-T(x_0) = 0$, implies the tension is constant.

$T u_x |_{x_0}^{x_1} =  \int_{x_0}^{x_1} \rho u_{tt} dx$

it implies,

$\frac{T u_x |_{x_0}^{x_1}}{x_1-x_0} =  \frac{\int_{x_0}^{x_1} \rho u_{tt}dx}{x_1 - x_0}$

As $x_1 \rightarrow x_0$, by (4) in preparatory, $Tu_{xx} =  \rho u_{tt}$

\subsubsection{Three variations of the equation}

As we can see there are three types of  equations: 


(1) $u_{tt} - c^2 u_{xx} + r u_t =0,r > 0$, when there is some air resistance. 


(2) $u_tt - c^2 u_{xx} + ku = 0, k > 0$, when there is an traverse elastic force proportional to the displacement $u$.

(3) $u_{tt}-c^2u_{xx} = f(x,t)$, if there is an extra force. 

Real life cases of the equations:

elastic bar, the sound waves in a pipe,  water waves in a striaght canal.

Electrical current in a transmission line with equation:

$$u_{xx} = CLu_{tt} + (CR+GL)u_t + GRu$$

C is the capacitance per unit length, G is the leakage resistance per unit, $R$ is the resistence per unition length, L is the self-inductance per unit length.

\subsection{Vibrating Drumhead}


$$\int_{\partial D} T \frac{\partial{u}}{\partial n} ds =\int\int_{D} \rho u_{tt} dx dy =ma$$ Why? On the page 14.

$\frac{\partial{u}}{\partial n} = n \cdot \nabla u$

$$\int_{\partial D}  (T\nabla u) \cdot n ds =\int\int_{D} \rho u_{tt} dx dy$$


By Green Theorem, which states,
$$\int_C f \cdot n ds = \int\int_D \nabla \cdot f  dxdy$$

$$\int\int_D \nabla \cdot(T\nabla u) dxdy =\int\int_{D} \rho u_{tt} dx dy$$

$$T \nabla \cdot(\nabla u)= \nabla \cdot(T\nabla u) = \rho u_{tt}$$

By Laplacian(\url{https://en.wikipedia.org/wiki/Laplace_operator}),

$$T(u_{xx}+u_{yy}) = \rho u_{tt}$$

Examples: free mesons in nuclear physics

\subsection{Diffusion}

\subsection{Heat Flow}

\subsection{Stationary Waves and Diffusions}

\subsection{The Hydrogen Atom}

\end{document}
